In Vale, add a sample memory-to-heaplet invariant (mem == heap0)

vale/code/arch/Vale.Arch.Heap.fst
@@ -2,6 +2,7 @@ module Vale.Arch.Heap
 open FStar.Mul
 open Vale.Interop
 open Vale.Arch.HeapImpl
+module Map16 = Vale.Lib.Map16
 friend Vale.Arch.HeapImpl
 
 let heap_impl = vale_full_heap
@@ -9,10 +10,15 @@ let heap_impl = vale_full_heap
 let heap_get hi = hi.vf_heap.mh
 
 let heap_upd hi mh' =
-  {vf_layout = hi.vf_layout; vf_heap = mi_heap_upd hi.vf_heap mh'; vf_heaplets = hi.vf_heaplets}
+  let h' = mi_heap_upd hi.vf_heap mh' in
+  {
+    vf_layout = hi.vf_layout;
+    vf_heap = h';
+    vf_heaplets = Map16.upd hi.vf_heaplets 0 h';
+  }
 
 let heap_create_from_interop ih =
   let vh = ValeHeap (down_mem ih) (Ghost.hide ih) in
   let vh4 = ((vh, vh), (vh, vh)) in
   let vh16 = ((vh4, vh4), (vh4, vh4)) in
-  {vf_layout = {vl_old_heap = vh}; vf_heap = vh; vf_heaplets = vh16}
+  {vf_layout = {vl_old_heap = vh}; vf_heap = vh; vf_heaplets = Map16.upd vh16 0 vh}
