vale/code/arch/x64/interop/Vale.X64.MemoryAdapters.fsti
@@ -2,6 +2,7 @@ module Vale.X64.MemoryAdapters
 
 open FStar.Mul
 open Vale.Interop.Base
+open Vale.Arch.HeapImpl
 module BS = Vale.X64.Machine_Semantics_s
 module BV = LowStar.BufferView
 module HS = FStar.HyperStack
@@ -10,6 +11,7 @@ module SI = Vale.X64.Stack_i
 module IB = Vale.Interop.Base
 module VS = Vale.X64.State
 module V = Vale.X64.Decls
+module Map16 = Vale.Lib.Map16
 val as_vale_buffer (#src #t:base_typ) (i:IB.buf_t src t) : GTot (ME.buffer t)
 val as_vale_immbuffer (#src #t:base_typ) (i:IB.ibuf_t src t) : GTot (ME.buffer t)
 
@@ -17,7 +19,9 @@ val stack_eq : squash (BS.machine_stack == SI.vale_stack)
 
 val as_mem (h:ME.vale_full_heap) : GTot IB.interop_heap
 
-val create_initial_vale_heap (ih:IB.interop_heap) : GTot ME.vale_full_heap
+val create_initial_vale_heap (ih:IB.interop_heap) : Ghost vale_full_heap
+  (requires True)
+  (ensures ME.mem_inv)
 
 unfold
 let as_vale_stack (st:BS.machine_stack)
