vale/specs/hardware/Vale.X64.Machine_Semantics_s.fst
@@ -501,7 +501,7 @@ let ins_obs (ins:ins) (s:machine_state) : list observation =
   | BC.Instr (InstrTypeRecord #outs #args _) oprs _ -> obs_inouts outs args oprs s
   | BC.Push src _ -> operand_obs s src
   | BC.Pop dst _ -> operand_obs s dst
-  | BC.Alloc _ | BC.Dealloc _ -> []
+  | BC.Alloc _ | BC.Dealloc _ | BC.HeapGhost _ -> []
 
 [@instr_attr]
 let instr_eval_operand_explicit (i:instr_operand_explicit) (o:instr_operand_t i) (s:machine_state) : option (instr_val_t (IOpEx i)) =
@@ -672,6 +672,9 @@ let machine_eval_ins_st (ins:ins) : st unit =
     update_rsp new_rsp;;
     // The deallocated stack memory should now be considered invalid
     free_stack old_rsp new_rsp
+
+  | BC.HeapGhost f ->
+    set ({s with ms_heap = f s.ms_heap})
 
 [@instr_attr]
 let machine_eval_ins (i:ins) (s:machine_state) : machine_state =
